Introduce extcall events and calling conventions

common/Events.v
@@ -24,6 +24,7 @@ Require Import Floats.
 Require Import Values.
 Require Import Memory.
 Require Import Globalenvs.
+Require Export LanguageInterface.
 
 (** * Events and traces *)
 
@@ -65,7 +66,8 @@ Inductive event: Type :=
   | Event_syscall: string -> list eventval -> eventval -> event
   | Event_vload: memory_chunk -> ident -> ptrofs -> eventval -> event
   | Event_vstore: memory_chunk -> ident -> ptrofs -> eventval -> event
-  | Event_annot: string -> list eventval -> event.
+  | Event_annot: string -> list eventval -> event
+  | Event_extcall: ident -> query -> reply -> event.
 
 (** The dynamic semantics for programs collect traces of events.
   Traces are of two kinds: finite (type [trace]) or infinite (type [traceinf]). *)
@@ -446,19 +448,7 @@ Section EVENTVAL_INJECT.
 Variable f: block -> option (block * Z).
 Variable ge1 ge2: Senv.t.
 
-Definition symbols_inject : Prop :=
-   (forall id, Senv.public_symbol ge2 id = Senv.public_symbol ge1 id)
-/\ (forall id b1 b2 delta,
-     f b1 = Some(b2, delta) -> Senv.find_symbol ge1 id = Some b1 ->
-     delta = 0 /\ Senv.find_symbol ge2 id = Some b2)
-/\ (forall id b1,
-     Senv.public_symbol ge1 id = true -> Senv.find_symbol ge1 id = Some b1 ->
-     exists b2, f b1 = Some(b2, 0) /\ Senv.find_symbol ge2 id = Some b2)
-/\ (forall b1 b2 delta,
-     f b1 = Some(b2, delta) ->
-     Senv.block_is_volatile ge2 b2 = Senv.block_is_volatile ge1 b1).
-
-Hypothesis symb_inj: symbols_inject.
+Hypothesis symb_inj: symbols_inject f ge1 ge2.
 
 Lemma eventval_match_inject:
   forall ev ty v1 v2,
@@ -495,11 +485,99 @@ End EVENTVAL_INJECT.
 Section MATCH_TRACES.
 
 Variable ge: Senv.t.
+Variable cc: callconv.
+Variable w: world cc.
 
 (** Matching between traces corresponding to single transitions.
-  Arguments (provided by the program) must be equal.
+  Arguments (provided by the program) must be related.
   Results (provided by the outside world) can vary as long as they
   can be converted safely to values. *)
+
+Inductive match_events_query: trace -> trace -> Prop :=
+  | match_events_query_E0:
+      match_events_query nil nil
+  | match_events_query_syscall id args res1 res2:
+      eventval_valid ge res1 ->
+      eventval_valid ge res2 ->
+      eventval_type res1 = eventval_type res2 ->
+      match_events_query
+        (Event_syscall id args res1 :: nil)
+        (Event_syscall id args res2 :: nil)
+  | match_events_query_vload chunk id ofs res1 res2:
+      eventval_valid ge res1 ->
+      eventval_valid ge res2 ->
+      eventval_type res1 = eventval_type res2 ->
+      match_events_query
+        (Event_vload chunk id ofs res1 :: nil)
+        (Event_vload chunk id ofs res2 :: nil)
+  | match_events_query_vstore chunk id ofs arg:
+      match_events_query
+        (Event_vstore chunk id ofs arg :: nil)
+        (Event_vstore chunk id ofs arg :: nil)
+  | match_events_query_annot id args:
+      match_events_query
+        (Event_annot id args :: nil)
+        (Event_annot id args :: nil)
+  | match_events_query_extcall f q1 q2 r1 r2:
+      extcall_valid q1 r1 ->
+      extcall_valid q2 r2 ->
+      match_query w q1 q2 ->
+      match_events_query
+        (Event_extcall f q1 r1 :: nil)
+        (Event_extcall f q2 r2 :: nil).
+
+Inductive match_events: trace -> trace -> Prop :=
+  | match_events_E0:
+      match_events nil nil
+  | match_events_syscall id args res:
+      eventval_valid ge res ->
+      match_events
+        (Event_syscall id args res :: nil)
+        (Event_syscall id args res :: nil)
+  | match_events_vload chunk id ofs res:
+      eventval_valid ge res ->
+      match_events
+        (Event_vload chunk id ofs res :: nil)
+        (Event_vload chunk id ofs res :: nil)
+  | match_events_vstore chunk id ofs arg:
+      match_events
+        (Event_vstore chunk id ofs arg :: nil)
+        (Event_vstore chunk id ofs arg :: nil)
+  | match_events_annot id args:
+      match_events
+        (Event_annot id args :: nil)
+        (Event_annot id args :: nil)
+  | match_events_extcall f q1 q2 r1 r2:
+      extcall_valid q1 r1 ->
+      extcall_valid q2 r2 ->
+      match_query w q1 q2 ->
+      match_reply w r1 r2 ->
+      match_events
+        (Event_extcall f q1 r1 :: nil)
+        (Event_extcall f q2 r2 :: nil).
+
+Lemma match_events_subrel_query t1 t2:
+  match_events t1 t2 ->
+  match_events_query t1 t2.
+Proof.
+  destruct 1; constructor; eauto.
+Qed.
+
+(** Stable events are invariant under the calling convention. *)
+
+Definition stable_event t :=
+  match t with
+    | nil => True
+    | Event_syscall _ _ res :: nil => eventval_valid ge res
+    | Event_vload _ _ _ res :: nil => eventval_valid ge res
+    | Event_extcall _ _ _ :: nil => False
+    | _ :: nil => True
+    | _ => False
+  end.
+
+(** For stable events, we can use the simpler [match_traces] below
+  instead of [match_events_query], and use equality instead of
+  [match_events]. *)
 
 Inductive match_traces: trace -> trace -> Prop :=
   | match_traces_E0:
@@ -513,7 +591,43 @@ Inductive match_traces: trace -> trace -> Prop :=
   | match_traces_vstore: forall chunk id ofs arg,
       match_traces (Event_vstore chunk id ofs arg :: nil) (Event_vstore chunk id ofs arg :: nil)
   | match_traces_annot: forall id args,
-      match_traces (Event_annot id args :: nil) (Event_annot id args :: nil).
+      match_traces (Event_annot id args :: nil) (Event_annot id args :: nil)
+  | match_traces_extcall: forall id q r1 r2,
+      extcall_valid q r1 ->
+      extcall_valid q r2 ->
+      match_traces (Event_extcall id q r1 :: nil) (Event_extcall id q r2 :: nil).
+
+Lemma match_traces_match_events_query t1 t2:
+  stable_event t1 ->
+  match_traces t1 t2 ->
+  match_events_query t1 t2.
+Proof.
+  destruct 2; try contradiction; constructor; auto.
+Qed.
+
+Lemma match_events_query_match_traces t1 t2:
+  stable_event t1 ->
+  match_events_query t1 t2 ->
+  match_traces t1 t2.
+Proof.
+  destruct 2; try contradiction; constructor; auto.
+Qed.
+
+Lemma match_stable_event_refl t:
+  stable_event t ->
+  match_events t t.
+Proof.
+  intros Ht.
+  destruct t as [ | [] []]; contradiction || constructor; auto.
+Qed.
+
+Lemma match_stable_event_corefl t1 t2:
+  stable_event t1 ->
+  match_events t1 t2 ->
+  t1 = t2.
+Proof.
+  destruct 2; tauto.
+Qed.
 
 End MATCH_TRACES.
 
@@ -522,14 +636,16 @@ End MATCH_TRACES.
 Section MATCH_TRACES_INV.
 
 Variables ge1 ge2: Senv.t.
+Variable cc: callconv.
+Variable w: world cc.
 
 Hypothesis public_preserved:
   forall id, Senv.public_symbol ge2 id = Senv.public_symbol ge1 id.
 
 Lemma match_traces_preserved:
-  forall t1 t2, match_traces ge1 t1 t2 -> match_traces ge2 t1 t2.
+  forall t1 t2, match_events_query ge1 w t1 t2 -> match_events_query ge2 w t1 t2.
 Proof.
-  induction 1; constructor; auto; eapply eventval_valid_preserved; eauto.
+  induction 1; econstructor; eauto using eventval_valid_preserved.
 Qed.
 
 End MATCH_TRACES_INV.
@@ -543,6 +659,7 @@ Definition output_event (ev: event) : Prop :=
   | Event_vload _ _ _ _ => False
   | Event_vstore _ _ _ _ => True
   | Event_annot _ _ => True
+  | Event_extcall _ _ _ => False
   end.
 
 Fixpoint output_trace (t: trace) : Prop :=
@@ -595,25 +712,82 @@ Inductive volatile_store (ge: Senv.t):
 Definition extcall_sem : Type :=
   Senv.t -> list val -> mem -> trace -> val -> mem -> Prop.
 
+(** External calls must commute with the calling convention, in the
+  following sense. The system has two responsabilities: when two
+  states are related by the simulation relation, the forward
+  simulation should hold on the system component of any generated
+  event (per [match_traces]). Receptiveness means that any environment
+  behavior will then be allowed. In the case where the source and
+  target environments have related behaviors (per [match_event]),
+  then the system needs to transition to related states. *)
+
+Record extcall_relational_properties cc (sem: extcall_sem) (sg: signature) :=
+  {
+    ec_query ge1 ge2 w vargs1 m1 t1 vres1 m1' vargs2 m2:
+      sem ge1 vargs1 m1 t1 vres1 m1' ->
+      match_senv w ge1 ge2 ->
+      match_query (cc:=cc) w (sg, vargs1, m1) (sg, vargs2, m2) ->
+      exists t2 vres2 m2',
+        sem ge2 vargs2 m2 t2 vres2 m2' /\
+        match_events_query ge1 w t1 t2;
+    ec_reply ge1 ge2 w vargs1 m1 t1 vres1 m1' vargs2 m2 t2:
+      sem ge1 vargs1 m1 t1 vres1 m1' ->
+      match_senv w ge1 ge2 ->
+      match_query w (sg, vargs1, m1) (sg, vargs2, m2) ->
+      match_events ge1 (cc:=cc) w t1 t2 ->
+      exists vres2 m2',
+        sem ge2 vargs2 m2 t2 vres2 m2' /\
+        match_reply w (vres1, m1') (vres2, m2');
+  }.
+
+(** For calls which generate stable events, [match_event] reduces to
+  equality, so that the two properties above collapse into one. *)
+
+Lemma extcall_stable_event_relational_properties cc (sem: extcall_sem) sg:
+  (forall ge1 ge2 w vargs m1 t vres m2 vargs' m1',
+    match_senv w ge1 ge2 ->
+    sem ge1 vargs m1 t vres m2 ->
+    match_query (cc:=cc) w (sg, vargs, m1) (sg, vargs', m1') ->
+    exists vres' m2',
+      sem ge2 vargs' m1' t vres' m2' /\ 
+      stable_event ge1 t /\
+      match_reply w (vres, m2) (vres', m2')) ->
+  extcall_relational_properties cc sem sg.
+Proof.
+  intros H.
+  split.
+  - intros until m2.
+    intros Hstep Hge Hq.
+    edestruct H as (vres2 & m2' & Hstep2 & Ht & Hr); eauto.
+    exists t1, vres2, m2'.
+    split; eauto.
+    eapply match_events_subrel_query.
+    eapply match_stable_event_refl; eauto.
+  - intros until t2.
+    intros Hstep1 Hge Hq Ht.
+    edestruct H as (vres2 & m2' & Hstep2 & Ht' & Hr); eauto.
+    assert (t1 = t2) by eauto using match_stable_event_corefl; subst t2.
+    exists vres2, m2'.
+    split; eauto.
+Qed.
+
+(** When proving [ec_mem_extends] or [ec_mem_inject] below, this can
+  be used for proofs of cases with stable events. We make some effort
+  to produce a proof state identical to before our changes. *)
+
+Ltac extcall_relational_properties_compat :=
+  eapply extcall_stable_event_relational_properties;
+  intros ge ge' w vargs m1 t vres m2 vargs' m1' Hge;
+  simpl in Hge; (subst ge' || rename Hge into H);
+  intro;
+  let Hq := fresh in
+  intros Hq **;
+  (eapply match_query_extends in Hq; destruct Hq as (? & ? & ?)) ||
+  (eapply match_query_inject in Hq; destruct Hq as (f & ? & ?& ?));
+  subst w;
+  simpl in *.
+
 (** We now specify the expected properties of this predicate. *)
-
-Definition loc_out_of_bounds (m: mem) (b: block) (ofs: Z) : Prop :=
-  ~Mem.perm m b ofs Max Nonempty.
-
-Definition loc_not_writable (m: mem) (b: block) (ofs: Z) : Prop :=
-  ~Mem.perm m b ofs Max Writable.
-
-Definition loc_unmapped (f: meminj) (b: block) (ofs: Z): Prop :=
-  f b = None.
-
-Definition loc_out_of_reach (f: meminj) (m: mem) (b: block) (ofs: Z): Prop :=
-  forall b0 delta,
-  f b0 = Some(b, delta) -> ~Mem.perm m b0 (ofs - delta) Max Nonempty.
-
-Definition inject_separated (f f': meminj) (m1 m2: mem): Prop :=
-  forall b1 b2 delta,
-  f b1 = None -> f' b1 = Some(b2, delta) ->
-  ~Mem.valid_block m1 b1 /\ ~Mem.valid_block m2 b2.
 
 Record extcall_properties (sem: extcall_sem) (sg: signature) : Prop :=
   mk_extcall_properties {
@@ -655,32 +829,12 @@ Record extcall_properties (sem: extcall_sem) (sg: signature) : Prop :=
 (** External calls must commute with memory extensions, in the
   following sense. *)
   ec_mem_extends:
-    forall ge vargs m1 t vres m2 m1' vargs',
-    sem ge vargs m1 t vres m2 ->
-    Mem.extends m1 m1' ->
-    Val.lessdef_list vargs vargs' ->
-    exists vres', exists m2',
-       sem ge vargs' m1' t vres' m2'
-    /\ Val.lessdef vres vres'
-    /\ Mem.extends m2 m2'
-    /\ Mem.unchanged_on (loc_out_of_bounds m1) m1' m2';
+    extcall_relational_properties cc_extends sem sg;
 
 (** External calls must commute with memory injections,
   in the following sense. *)
   ec_mem_inject:
-    forall ge1 ge2 vargs m1 t vres m2 f m1' vargs',
-    symbols_inject f ge1 ge2 ->
-    sem ge1 vargs m1 t vres m2 ->
-    Mem.inject f m1 m1' ->
-    Val.inject_list f vargs vargs' ->
-    exists f', exists vres', exists m2',
-       sem ge2 vargs' m1' t vres' m2'
-    /\ Val.inject f' vres vres'
-    /\ Mem.inject f' m2 m2'
-    /\ Mem.unchanged_on (loc_unmapped f) m1 m2
-    /\ Mem.unchanged_on (loc_out_of_reach f m1) m1' m2'
-    /\ inject_incr f f'
-    /\ inject_separated f f' m1 m1';
+    extcall_relational_properties cc_inject sem sg;
 
 (** External calls produce at most one event. *)
   ec_trace_length:
@@ -785,14 +939,17 @@ Proof.
 (* readonly *)
 - inv H. apply Mem.unchanged_on_refl.
 (* mem extends *)
-- inv H. inv H1. inv H6. inv H4.
+- extcall_relational_properties_compat.
+  inv H. inv H1. inv H6. inv H4.
   exploit volatile_load_extends; eauto. intros [v' [A B]].
   exists v'; exists m1'; intuition. constructor; auto.
+  admit. (* volatile load has stable event *)
 (* mem injects *)
-- inv H0. inv H2. inv H7. inversion H5; subst.
+- extcall_relational_properties_compat.
+  inv H0. inv H2. inv H7. inversion H5; subst.
   exploit volatile_load_inject; eauto. intros [v' [A B]].
-  exists f; exists v'; exists m1'; intuition. constructor; auto.
-  red; intros. congruence.
+  exists v'; exists m1'; intuition. constructor; auto.
+  admit. (* stable event *)
 (* trace length *)
 - inv H; inv H0; simpl; omega.
 (* receptive *)
@@ -809,7 +966,7 @@ Proof.
   assert (v = v0) by (eapply eventval_match_determ_1; eauto). subst v0.
   auto.
   split. constructor. intuition congruence.
-Qed.
+Admitted.
 
 (** ** Semantics of volatile stores *)
 
@@ -855,7 +1012,7 @@ Lemma volatile_store_extends:
   /\ Mem.extends m2 m2'
   /\ Mem.unchanged_on (loc_out_of_bounds m1) m1' m2'.
 Proof.
-  intros. inv H.
+  intros. inv H; inv H2.
 - econstructor; split. econstructor; eauto.
   eapply eventval_match_lessdef; eauto. apply Val.load_result_lessdef; auto.
   auto with mem.
@@ -935,13 +1092,18 @@ Proof.
 (* readonly *)
 - inv H. eapply volatile_store_readonly; eauto.
 (* mem extends*)
-- inv H. inv H1. inv H6. inv H7. inv H4.
+- extcall_relational_properties_compat.
+  inv H. inv H1. inv H6. inv H7. inv H4.
   exploit volatile_store_extends; eauto. intros [m2' [A [B C]]].
   exists Vundef; exists m2'; intuition. constructor; auto.
+  admit. (* stable event *)
 (* mem inject *)
-- inv H0. inv H2. inv H7. inv H8. inversion H5; subst.
+- extcall_relational_properties_compat.
+  inv H0. inv H2. inv H7. inv H8. inversion H5; subst.
   exploit volatile_store_inject; eauto. intros [m2' [A [B [C D]]]].
-  exists f; exists Vundef; exists m2'; intuition. constructor; auto. red; intros; congruence.
+  exists Vundef; exists m2'; intuition. constructor; auto.
+  admit. (* stable event *)
+  eapply match_reply_inject_intro; eauto.
 (* trace length *)
 - inv H; inv H0; simpl; omega.
 (* receptive *)
@@ -953,7 +1115,7 @@ Proof.
   assert (ev = ev0) by (eapply eventval_match_determ_2; eauto). subst ev0.
   split. constructor. auto.
   split. constructor. intuition congruence.
-Qed.
+Admitted.
 
 (** ** Semantics of dynamic memory allocation (malloc) *)
 
@@ -995,7 +1157,8 @@ Proof.
 (* readonly *)
 - inv H. eapply UNCHANGED; eauto.
 (* mem extends *)
-- inv H. inv H1. inv H7.
+- extcall_relational_properties_compat.
+  inv H. inv H1. inv H7.
   assert (SZ: v2 = Vptrofs sz).
   { unfold Vptrofs in *. destruct Archi.ptr64; inv H5; auto. }
   subst v2.
@@ -1005,9 +1168,11 @@ Proof.
   intros [m2' [C D]].
   exists (Vptr b Ptrofs.zero); exists m2'; intuition.
   econstructor; eauto.
-  eapply UNCHANGED; eauto.
+  admit. (* stable event *)
+  eauto.
 (* mem injects *)
-- inv H0. inv H2. inv H8.
+- extcall_relational_properties_compat.
+  inv H0. inv H2. inv H8.
   assert (SZ: v' = Vptrofs sz).
   { unfold Vptrofs in *. destruct Archi.ptr64; inv H6; auto. }
   subst v'.
@@ -1016,11 +1181,10 @@ Proof.
   exploit Mem.store_mapped_inject. eexact A. eauto. eauto.
   instantiate (1 := Vptrofs sz). unfold Vptrofs; destruct Archi.ptr64; constructor.
   rewrite Zplus_0_r. intros [m2' [E G]].
-  exists f'; exists (Vptr b' Ptrofs.zero); exists m2'; intuition auto.
+  exists (Vptr b' Ptrofs.zero); exists m2'; intuition auto.
   econstructor; eauto.
-  econstructor. eauto. auto.
-  eapply UNCHANGED; eauto.
-  eapply UNCHANGED; eauto.
+  admit. (* stable event *)
+  eapply match_reply_inject_intro; eauto.
   red; intros. destruct (eq_block b1 b).
   subst b1. rewrite C in H2. inv H2. eauto with mem.
   rewrite D in H2 by auto. congruence.
@@ -1038,7 +1202,7 @@ Proof.
   }
   subst.
   split. constructor. intuition congruence.
-Qed.
+Admitted.
 
 (** ** Semantics of dynamic memory deallocation (free) *)
 
@@ -1069,7 +1233,8 @@ Proof.
   apply Mem.perm_cur_max. apply Mem.perm_implies with Freeable; auto with mem.
   eapply Mem.free_range_perm; eauto.
 (* mem extends *)
-- inv H. inv H1. inv H8. inv H6.
+- extcall_relational_properties_compat.
+  inv H. inv H1. inv H8. inv H6.
   exploit Mem.load_extends; eauto. intros [v' [A B]].
   assert (v' = Vptrofs sz).
   { unfold Vptrofs in *; destruct Archi.ptr64; inv B; auto. }
@@ -1077,6 +1242,8 @@ Proof.
   exploit Mem.free_parallel_extends; eauto. intros [m2' [C D]].
   exists Vundef; exists m2'; intuition.
   econstructor; eauto.
+  simpl. auto.
+  eapply match_reply_extends_intro; eauto.
   eapply Mem.free_unchanged_on; eauto.
   unfold loc_out_of_bounds; intros.
   assert (Mem.perm m1 b i Max Nonempty).
@@ -1084,7 +1251,8 @@ Proof.
     eapply Mem.free_range_perm. eexact H4. eauto. }
   tauto.
 (* mem inject *)
-- inv H0. inv H2. inv H7. inv H9.
+- extcall_relational_properties_compat.
+  inv H0. inv H2. inv H7. inv H9.
   exploit Mem.load_inject; eauto. intros [v' [A B]].
   assert (v' = Vptrofs sz).
   { unfold Vptrofs in *; destruct Archi.ptr64; inv B; auto. }
@@ -1097,20 +1265,18 @@ Proof.
     generalize (size_chunk_pos Mptr); omega.
   intro EQ.
   exploit Mem.free_parallel_inject; eauto. intros (m2' & C & D).
-  exists f, Vundef, m2'; split.
+  exists Vundef, m2'; split.
   apply extcall_free_sem_intro with (sz := sz) (m' := m2').
     rewrite EQ. rewrite <- A. f_equal. omega.
     auto. auto.
     rewrite ! EQ. rewrite <- C. f_equal; omega.
-  split. auto.
-  split. auto.
-  split. eapply Mem.free_unchanged_on; eauto. unfold loc_unmapped. intros; congruence.
-  split. eapply Mem.free_unchanged_on; eauto. unfold loc_out_of_reach.
+  simpl. split; auto.
+  eapply match_reply_inject_intro; eauto.
+  eapply Mem.free_unchanged_on; eauto. unfold loc_unmapped. intros; congruence.
+  eapply Mem.free_unchanged_on; eauto. unfold loc_out_of_reach.
     intros. red; intros. eelim H2; eauto.
     apply Mem.perm_cur_max. apply Mem.perm_implies with Freeable; auto with mem.
     apply P. omega.
-  split. auto.
-  red; intros. congruence.
 (* trace length *)
 - inv H; simpl; omega.
 (* receptive *)
@@ -1162,6 +1328,7 @@ Proof.
   intros; red; intros. elim H8.
   apply Mem.perm_cur_max. eapply Mem.storebytes_range_perm; eauto.
 - (* extensions *)
+  extcall_relational_properties_compat.
   intros. inv H.
   inv H1. inv H13. inv H14. inv H10. inv H11.
   exploit Mem.loadbytes_length; eauto. intros LEN.
@@ -1170,7 +1337,7 @@ Proof.
   exists Vundef; exists m2'.
   split. econstructor; eauto.
   split. constructor.
-  split. auto.
+  apply match_reply_extends_intro; auto.
   eapply Mem.storebytes_unchanged_on; eauto. unfold loc_out_of_bounds; intros.
   assert (Mem.perm m1 bdst i Max Nonempty).
   apply Mem.perm_cur_max. apply Mem.perm_implies with Writable; auto with mem.
@@ -1178,6 +1345,7 @@ Proof.
   erewrite list_forall2_length; eauto.
   tauto.
 - (* injections *)
+  extcall_relational_properties_compat.
   intros. inv H0. inv H2. inv H14. inv H15. inv H11. inv H12.
   destruct (zeq sz 0).
 + (* special case sz = 0 *)
@@ -1187,20 +1355,19 @@ Proof.
   destruct (Mem.range_perm_storebytes m1' b0 (Ptrofs.unsigned (Ptrofs.add odst (Ptrofs.repr delta0))) nil)
   as [m2' SB].
   simpl. red; intros; omegaContradiction.
-  exists f, Vundef, m2'.
+  exists Vundef, m2'.
   split. econstructor; eauto.
   intros; omegaContradiction.
   intros; omegaContradiction.
   right; omega.
   apply Mem.loadbytes_empty. omega.
-  split. auto.
-  split. eapply Mem.storebytes_empty_inject; eauto.
-  split. eapply Mem.storebytes_unchanged_on; eauto. unfold loc_unmapped; intros.
+  split. constructor.
+  eapply match_reply_inject_intro; eauto.
+  eapply Mem.storebytes_empty_inject; eauto.
+  eapply Mem.storebytes_unchanged_on; eauto. unfold loc_unmapped; intros.
   congruence.
-  split. eapply Mem.storebytes_unchanged_on; eauto.
+  eapply Mem.storebytes_unchanged_on; eauto.
   simpl; intros; omegaContradiction.
-  split. apply inject_incr_refl.
-  red; intros; congruence.
 + (* general case sz > 0 *)
   exploit Mem.loadbytes_length; eauto. intros LEN.
   assert (RPSRC: Mem.range_perm m1 bsrc (Ptrofs.unsigned osrc) (Ptrofs.unsigned osrc + sz) Cur Nonempty).
@@ -1217,7 +1384,7 @@ Proof.
   exploit Mem.address_inject.  eauto. eexact PDST. eauto. intros EQ2.
   exploit Mem.loadbytes_inject; eauto. intros [bytes2 [A B]].
   exploit Mem.storebytes_mapped_inject; eauto. intros [m2' [C D]].
-  exists f; exists Vundef; exists m2'.
+  exists Vundef; exists m2'.
   split. econstructor; try rewrite EQ1; try rewrite EQ2; eauto.
   intros; eapply Mem.aligned_area_inject with (m := m1); eauto.
   intros; eapply Mem.aligned_area_inject with (m := m1); eauto.
@@ -1225,17 +1392,15 @@ Proof.
   apply Mem.range_perm_max with Cur; auto.
   apply Mem.range_perm_max with Cur; auto. omega.
   split. constructor.
-  split. auto.
-  split. eapply Mem.storebytes_unchanged_on; eauto. unfold loc_unmapped; intros.
+  eapply match_reply_inject_intro; eauto.
+  eapply Mem.storebytes_unchanged_on; eauto. unfold loc_unmapped; intros.
   congruence.
-  split. eapply Mem.storebytes_unchanged_on; eauto. unfold loc_out_of_reach; intros. red; intros.
+  eapply Mem.storebytes_unchanged_on; eauto. unfold loc_out_of_reach; intros. red; intros.
   eelim H2; eauto.
   apply Mem.perm_cur_max. apply Mem.perm_implies with Writable; auto with mem.
   eapply Mem.storebytes_range_perm; eauto.
   erewrite list_forall2_length; eauto.
   omega.
-  split. apply inject_incr_refl.
-  red; intros; congruence.
 - (* trace length *)
   intros; inv H. simpl; omega.
 - (* receptive *)
@@ -1272,16 +1437,19 @@ Proof.
 (* readonly *)
 - inv H. apply Mem.unchanged_on_refl.
 (* mem extends *)
-- inv H.
+- extcall_relational_properties_compat.
+  inv H.
   exists Vundef; exists m1'; intuition.
   econstructor; eauto.
   eapply eventval_list_match_lessdef; eauto.
+  constructor.
 (* mem injects *)
-- inv H0.
-  exists f; exists Vundef; exists m1'; intuition.
+- extcall_relational_properties_compat.
+  inv H0.
+  exists Vundef; exists m1'; intuition.
   econstructor; eauto.
   eapply eventval_list_match_inject; eauto.
-  red; intros; congruence.
+  constructor.
 (* trace length *)
 - inv H; simpl; omega.
 (* receptive *)
@@ -1317,16 +1485,19 @@ Proof.
 (* readonly *)
 - inv H. apply Mem.unchanged_on_refl.
 (* mem extends *)
-- inv H. inv H1. inv H6.
+- extcall_relational_properties_compat.
+  inv H. inv H1. inv H6.
   exists v2; exists m1'; intuition.
   econstructor; eauto.
   eapply eventval_match_lessdef; eauto.
+  constructor.
 (* mem inject *)
-- inv H0. inv H2. inv H7.
-  exists f; exists v'; exists m1'; intuition.
+- extcall_relational_properties_compat.
+  inv H0. inv H2. inv H7.
+  exists v'; exists m1'; intuition.
   econstructor; eauto.
   eapply eventval_match_inject; eauto.
-  red; intros; congruence.
+  constructor.
 (* trace length *)
 - inv H; simpl; omega.
 (* receptive *)
@@ -1360,14 +1531,17 @@ Proof.
 (* readonly *)
 - inv H. apply Mem.unchanged_on_refl.
 (* mem extends *)
-- inv H.
+- extcall_relational_properties_compat.
+  inv H.
   exists Vundef; exists m1'; intuition.
   econstructor; eauto.
+  constructor.
 (* mem injects *)
-- inv H0.
-  exists f; exists Vundef; exists m1'; intuition.
+- extcall_relational_properties_compat.
+  inv H0.
+  exists Vundef; exists m1'; intuition.
   econstructor; eauto.
-  red; intros; congruence.
+  constructor.
 (* trace length *)
 - inv H; simpl; omega.
 (* receptive *)
@@ -1380,16 +1554,79 @@ Qed.
 (** ** Semantics of external functions. *)
 
 (** For functions defined outside the program ([EF_external],
-  [EF_builtin] and [EF_runtime]), we do not define their
-  semantics, but only assume that it satisfies
-  [extcall_properties]. *)
+  [EF_builtin] and [EF_runtime]), we record an external call event. *)
 
-Parameter external_functions_sem: String.string -> signature -> extcall_sem.
+Inductive external_functions_sem id (sg: signature): extcall_sem :=
+  external_funcions_sem_intro ge vargs m vres m':
+    extcall_step_valid sg vargs m vres m' ->
+    external_functions_sem id sg ge vargs m (Event_extcall id (sg, vargs, m) (vres, m') :: E0) vres m'.
 
-Axiom external_functions_properties:
+Lemma external_functions_sem_relational_properties cc id sg:
+  extcall_relational_properties cc (external_functions_sem id sg) sg.
+Proof.
+  split.
+  - intros.
+    destruct H.
+    assert (Hvalid2: extcall_step_valid sg vargs2 m2 Vundef m2).
+    {
+      split; eauto.
+      + constructor.
+      + apply Mem.unchanged_on_refl.
+    }
+    eexists.
+    exists Vundef, m2.
+    split.
+    + econstructor; eauto.
+    + econstructor; eauto.
+  - intros.
+    destruct H.
+    inv H2.
+    assert (q2 = (sg, vargs2, m2)) by eauto using match_query_injective; subst.
+    destruct r2 as [vres2 m2'].
+    exists vres2, m2'.
+    split; eauto.
+    constructor; eauto.
+Qed.
+
+Lemma external_functions_properties:
   forall id sg, extcall_properties (external_functions_sem id sg) sg.
+Proof.
+  split.
+  (* well-typed *)
+  - destruct 1.
+    eapply ecv_well_typed; eauto.
+  (* symbols *)
+  - destruct 2; constructor; eauto.
+  (* valid blocks *)
+  - destruct 1.
+    eapply ecv_valid_block; eauto.
+  (* perms *)
+  - destruct 1.
+    eapply ecv_max_perm; eauto.
+  (* readonly *)
+  - destruct 1.
+    eapply ecv_readonly; eauto.
+  (* mem extends *)
+  - apply external_functions_sem_relational_properties.
+  (* mem inject *)
+  - apply external_functions_sem_relational_properties.
+  (* trace length *)
+  - destruct 1; simpl.
+    reflexivity.
+  (* receptive *)
+  - destruct 1; inversion 1.
+    destruct r2 as [vres2 m2].
+    exists vres2, m2.
+    constructor; auto.
+  (* determ *)
+  - destruct 1; inversion 1; subst.
+    split.
+    + constructor; eauto.
+    + inversion 1; auto.
+Qed.
 
-(** We treat inline assembly similarly. *)
+(** For inline assembly, we do not define its semantics,
+  but only assume that it satisfies [extcall_properties]. *)
 
 Parameter inline_assembly_sem: String.string -> signature -> extcall_sem.
 
@@ -1475,6 +1712,7 @@ Definition meminj_preserves_globals (F V: Type) (ge: Genv.t F V) (f: block -> op
   /\ (forall b gv, Genv.find_var_info ge b = Some gv -> f b = Some(b, 0))
   /\ (forall b1 b2 delta gv, Genv.find_var_info ge b2 = Some gv -> f b1 = Some(b2, delta) -> b2 = b1).
 
+(*
 Lemma external_call_mem_inject:
   forall ef F V (ge: Genv.t F V) vargs m1 t vres m2 f m1' vargs',
   meminj_preserves_globals ge f ->
@@ -1501,6 +1739,7 @@ Proof.
     * destruct (Genv.find_var_info ge b2) as [gv2|] eqn:V2; auto.
       exploit C; eauto. intros EQ; subst b2. congruence.
 Qed.
+*)
 
 (** Corollaries of [external_call_determ]. *)
 
