common/LanguageInterface.v
@@ -1,0 +1,284 @@
+Require Import Coqlib.
+Require Import AST.
+Require Import Integers.
+Require Import Floats.
+Require Import Values.
+Require Import Memory.
+Require Import Globalenvs.
+
+Set Implicit Arguments.
+
+(** * Semantic interface of languages *)
+
+Definition query: Type := signature * list val * mem.
+Definition reply: Type := val * mem.
+
+
+(** * Calling conventions *)
+
+Record callconv :=
+  mk_callconv {
+    world_def: Type;
+    match_senv_def:
+      world_def ->
+      Senv.t ->
+      Senv.t ->
+      Prop;
+    match_query_def:
+      world_def -> signature ->
+      list val -> mem ->
+      list val -> mem ->
+      Prop;
+    match_reply_def:
+      world_def -> signature ->
+      list val -> mem -> val -> mem ->
+      list val -> mem -> val -> mem ->
+      Prop;
+  }.
+
+Record world (cc: callconv) :=
+  mk_world {
+    cc_world :> world_def cc;
+    world_sg: signature;
+    world_sargs: list val;
+    world_smem: mem;
+    world_targs: list val;
+    world_tmem: mem;
+  }.
+
+Definition match_senv cc (w: world cc) (ge1 ge2: Senv.t): Prop :=
+  match_senv_def cc w ge1 ge2.
+
+Inductive match_query cc: world cc -> query -> query -> Prop :=
+  match_query_intro w sg vargs1 m1 vargs2 m2:
+    match_query_def cc w sg vargs1 m1 vargs2 m2 ->
+    match_query
+      (mk_world cc w sg vargs1 m1 vargs2 m2)
+      (sg, vargs1, m1)
+      (sg, vargs2, m2).
+
+Inductive match_reply cc: world cc -> reply -> reply -> Prop :=
+  match_reply_intro w sg vargs1 m1 vres1 m1' vargs2 m2 vres2 m2':
+    match_reply_def cc w sg vargs1 m1 vres1 m1' vargs2 m2 vres2 m2' ->
+    match_reply
+      (mk_world cc w sg vargs1 m1 vargs2 m2)
+      (vres1, m1')
+      (vres2, m2').
+
+Lemma match_query_injective cc (w: world cc) q q1 q2:
+  match_query w q q1 ->
+  match_query w q q2 ->
+  q1 = q2.
+Proof.
+  destruct 1.
+  inversion 1.
+  reflexivity.
+Qed.
+
+(** ** Expected properties of external call steps *)
+
+Definition loc_not_writable (m: mem) (b: block) (ofs: Z) : Prop :=
+  ~Mem.perm m b ofs Max Writable.
+
+Record extcall_step_valid sg (vargs: list val) m1 vres m2 :=
+  {
+    ecv_well_typed:
+      Val.has_type vres (proj_sig_res sg);
+    ecv_valid_block b:
+      Mem.valid_block m1 b ->
+      Mem.valid_block m2 b;
+    ecv_max_perm b ofs p:
+      Mem.valid_block m1 b ->
+      Mem.perm m2 b ofs Max p ->
+      Mem.perm m1 b ofs Max p;
+    ecv_readonly:
+      Mem.unchanged_on (loc_not_writable m1) m1 m2;
+  }.
+
+Definition extcall_valid (q: query) (r: reply) :=
+  let '(sg, vargs, m) := q in
+  let '(vres, m') := r in
+  extcall_step_valid sg vargs m vres m'.
+
+(** ** Equality passes *)
+
+Definition cc_id :=
+  {|
+    world_def := unit;
+    match_senv_def w := eq;
+    match_query_def w sg vargs1 m1 vargs2 m2 :=
+      vargs1 = vargs2 /\ m1 = m2;
+    match_reply_def w sg vargs1 m1 vres1 m1' vargs2 m2 vres2 m2' :=
+      vres1 = vres2 /\ m1' = m2';
+  |}.
+
+(** ** Extension passes *)
+
+Definition loc_out_of_bounds (m: mem) (b: block) (ofs: Z) : Prop :=
+  ~Mem.perm m b ofs Max Nonempty.
+
+Definition cc_extends :=
+  {|
+    world_def := unit;
+    match_senv_def w := eq;
+    match_query_def w sg vargs1 m1 vargs2 m2 :=
+      Val.lessdef_list vargs1 vargs2 /\
+      Mem.extends m1 m2;
+    match_reply_def w sg vargs1 m1 vres1 m1' vargs2 m2 vres2 m2' :=
+      Val.lessdef vres1 vres2 /\
+      Mem.extends m1' m2' /\
+      Mem.unchanged_on (loc_out_of_bounds m1) m2 m2';
+  |}.
+
+Lemma match_query_extends w sg vargs1 m1 vargs2 m2:
+  match_query (cc := cc_extends) w (sg, vargs1, m1) (sg, vargs2, m2) ->
+  Mem.extends m1 m2 /\
+  Val.lessdef_list vargs1 vargs2 /\
+  w = mk_world cc_extends tt sg vargs1 m1 vargs2 m2.
+Proof.
+  inversion 1; subst.
+  destruct H2, w0.
+  eauto.
+Qed.
+
+Lemma match_query_extends_intro sg vargs1 m1 vargs2 m2:
+  Mem.extends m1 m2 ->
+  Val.lessdef_list vargs1 vargs2 ->
+  match_query
+    (mk_world cc_extends tt sg vargs1 m1 vargs2 m2)
+    (sg, vargs1, m1)
+    (sg, vargs2, m2).
+Proof.
+  constructor.
+  simpl.
+  tauto.
+Qed.
+
+Lemma match_reply_extends_intro sg vargs1 m1 vres1 m1' vargs2 m2 vres2 m2':
+  Val.lessdef vres1 vres2 ->
+  Mem.extends m1' m2' ->
+  Mem.unchanged_on (loc_out_of_bounds m1) m2 m2' ->
+  match_reply
+    (mk_world cc_extends tt sg vargs1 m1 vargs2 m2)
+    (vres1, m1')
+    (vres2, m2').
+Proof.
+  intros Hvres Hm' Hm2.
+  constructor; simpl; auto.
+Qed.
+
+Hint Resolve match_query_extends_intro match_reply_extends_intro.
+
+(** ** Injection passes *)
+
+Definition symbols_inject (f: meminj) (ge1 ge2: Senv.t): Prop :=
+   (forall id, Senv.public_symbol ge2 id = Senv.public_symbol ge1 id)
+/\ (forall id b1 b2 delta,
+     f b1 = Some(b2, delta) -> Senv.find_symbol ge1 id = Some b1 ->
+     delta = 0 /\ Senv.find_symbol ge2 id = Some b2)
+/\ (forall id b1,
+     Senv.public_symbol ge1 id = true -> Senv.find_symbol ge1 id = Some b1 ->
+     exists b2, f b1 = Some(b2, 0) /\ Senv.find_symbol ge2 id = Some b2)
+/\ (forall b1 b2 delta,
+     f b1 = Some(b2, delta) ->
+     Senv.block_is_volatile ge2 b2 = Senv.block_is_volatile ge1 b1).
+
+Definition loc_unmapped (f: meminj) (b: block) (ofs: Z): Prop :=
+  f b = None.
+
+Definition loc_out_of_reach (f: meminj) (m: mem) (b: block) (ofs: Z): Prop :=
+  forall b0 delta,
+  f b0 = Some(b, delta) -> ~Mem.perm m b0 (ofs - delta) Max Nonempty.
+
+Definition inject_separated (f f': meminj) (m1 m2: mem): Prop :=
+  forall b1 b2 delta,
+  f b1 = None -> f' b1 = Some(b2, delta) ->
+  ~Mem.valid_block m1 b1 /\ ~Mem.valid_block m2 b2.
+
+Definition cc_inject :=
+  {|
+    world_def := meminj;
+    match_senv_def := symbols_inject;
+    match_query_def f sg vargs1 m1 vargs2 m2 :=
+      Val.inject_list f vargs1 vargs2 /\
+      Mem.inject f m1 m2;
+    match_reply_def f sg vargs1 m1 vres1 m1' vargs2 m2 vres2 m2' :=
+      exists f',
+        Val.inject f' vres1 vres2 /\
+        Mem.inject f' m1' m2' /\
+        Mem.unchanged_on (loc_unmapped f) m1 m1' /\
+        Mem.unchanged_on (loc_out_of_reach f m1) m2 m2' /\
+        inject_incr f f' /\
+        inject_separated f f' m1 m2;
+  |}.
+
+Lemma match_query_inject w sg vargs1 m1 vargs2 m2:
+  match_query w (sg, vargs1, m1) (sg, vargs2, m2) ->
+  exists f,
+    Mem.inject f m1 m2 /\
+    Val.inject_list f vargs1 vargs2 /\
+    w = mk_world cc_inject f sg vargs1 m1 vargs2 m2.
+Proof.
+  inversion 1; subst.
+  simpl in *.
+  destruct H2.
+  eauto.
+Qed.
+
+Lemma match_query_inject_intro f sg vargs1 m1 vargs2 m2:
+  Val.inject_list f vargs1 vargs2 ->
+  Mem.inject f m1 m2 ->
+  match_query
+    (mk_world cc_inject f sg vargs1 m1 vargs2 m2)
+    (sg, vargs1, m1)
+    (sg, vargs2, m2).
+Proof.
+  constructor.
+  simpl.
+  tauto.
+Qed.
+
+Lemma match_reply_inject_intro f f' sg vargs1 m1 vres1 m1' vargs2 m2 vres2 m2':
+  Mem.inject f' m1' m2' ->
+  Val.inject f' vres1 vres2 ->
+  Mem.unchanged_on (loc_unmapped f) m1 m1' ->
+  Mem.unchanged_on (loc_out_of_reach f m1) m2 m2' ->
+  inject_incr f f' ->
+  inject_separated f f' m1 m2 ->
+  match_reply
+    (mk_world cc_inject f sg vargs1 m1 vargs2 m2)
+    (vres1, m1')
+    (vres2, m2').
+Proof.
+  constructor; simpl; eauto 10.
+Qed.
+
+Lemma match_reply_inject_intro_same f sg vargs1 m1 vres1 vargs2 m2 vres2:
+  Mem.inject f m1 m2 ->
+  Val.inject f vres1 vres2 ->
+  match_reply
+    (mk_world cc_inject f sg vargs1 m1 vargs2 m2)
+    (vres1, m1)
+    (vres2, m2).
+Proof.
+  intros Hm Hvres.
+  constructor; simpl.
+  exists f; intuition.
+  intros b1 b2 delta Hb1 Hb1'.
+  congruence.
+Qed.
+
+Hint Resolve match_query_inject_intro.
+Hint Resolve match_reply_inject_intro.
+Hint Resolve match_reply_inject_intro_same.
+
+(** This is usedful as a hint to resolve the premices of
+  [match_reply_inject_intro]. *)
+
+Lemma same_inject_separated f m1 m2:
+  inject_separated f f m1 m2.
+Proof.
+  congruence.
+Qed.
+
+Hint Resolve same_inject_separated.
